Add PBOS equipped with a counter

CE_PBOS.v
@@ -345,3 +345,289 @@ Theorem peval_list_determinism :
 Proof.
   apply peval_determinism.
 Qed.
+
+
+
+Reserved Notation "| env , id , e , eff , counter | -aa> | id' , e' , eff' |" (at level 70).
+Reserved Notation "| env , id , e , eff ,  counter  | -pp> | id' , e' , eff' |" (at level 70).
+Reserved Notation "| env , id , e , eff ,  counter  | -ll> | id' , e' , eff' |" (at level 70).
+Inductive ppeval_aux : Environment -> nat -> AuxExpression -> SideEffectList -> nat -> nat -> Value + Exception -> SideEffectList -> Prop :=
+
+| ppeval_app1_exc env id ex eff params n:
+  |env, id, AApp1 (inr ex) params, eff, S n | -aa> |id, inr ex, eff|
+
+| ppeval_app1_fin env id id' id'' v eff eff' eff'' params res res' n:
+  |env, id, AList params (inl []), eff, n| -ll> |id', res, eff'| ->
+  |env, id', AApp2 v res, eff', n | -aa> |id'', res', eff'' |
+->
+  |env, id, AApp1 (inl v) params, eff, S n | -aa> |id'', res', eff''|
+
+| ppeval_app2_fin env id id' vals eff eff' res ref ext nid var_list body n:
+  length var_list = length vals ->
+  |append_vars_to_env var_list vals (get_env ref ext), id, body, eff, n| -pp> |id', res, eff'|
+->
+  |env, id, AApp2 (VClos ref ext nid var_list body) (inl vals), eff, S n| -aa> |id', res, eff'|
+
+| ppeval_app2_exc1 env id eff vals v n :
+  (forall ref ext var_list body n, v <> VClos ref ext n var_list body)
+->
+  |env, id, AApp2 v (inl vals), eff, S n| -aa> |id, inr (badfun v), eff|
+
+| ppeval_app2_exc2 env id eff var_list vals ref ext body nid n :
+  length var_list <> length vals
+->
+  | env, id, AApp2 (VClos ref ext nid var_list body) (inl vals), eff, S n | -aa> |id, inr (badarity (VClos ref ext nid var_list body)), eff|
+
+| ppeval_app2_exc env id eff v ex n:
+  |env, id, AApp2 v (inr ex), eff, S n| -aa> |id, inr ex, eff|
+
+| ppeval_let_exc env id v ex e2 eff n:
+  | env, id, ALet v (inr ex) e2, eff, S n | -aa> | id, inr ex, eff |
+
+| ppeval_let_fin env var v e2 eff id id' eff' res n:
+  | insert_value env (inl var) v, id, e2, eff, n| -pp> | id', res, eff' |
+->
+  | env, id, ALet var (inl v) e2, eff, S n | -aa> | id', res, eff' |
+
+| ppeval_call_fin env id f vals eff eff' res n:
+  eval f vals eff = (res, eff')
+->
+  | env, id, ACall f (inl vals), eff , S n| -aa> | id, res, eff' |
+
+| ppeval_call_exc env id f eff ex n:
+  | env, id, ACall f (inr ex), eff , S n| -aa> | id, inr ex, eff |
+
+| ppeval_try1_fin env id id' eff eff' v v1 e2 e3 varl res n:
+  |insert_value env (inl v1) v, id, e2, eff, n | -pp> | id', res, eff'|
+->
+  | env, id, ATry (inl v) v1 e2 varl e3, eff, S n | -aa> | id', res, eff'|
+
+| ppeval_try1_exc env id id' eff eff' ex v1 e2 e3 varl res n:
+  |append_try_vars_to_env varl [exclass_to_value (fst (fst ex)); snd (fst ex); snd ex] env, id, e3, eff, n|
+ -pp>
+  |id', res, eff'|
+->
+  | env, id, ATry (inr ex) v1 e2 varl e3, eff, S n | -aa> | id', res, eff'|
+
+where "| env , id , e , eff , counter | -aa> | id' , e' , eff' |" := (ppeval_aux env id e eff counter id' e' eff')
+with ppeval_expr : Environment -> nat -> Expression -> SideEffectList -> nat -> nat -> Value + Exception -> SideEffectList -> Prop :=
+
+(* literal evaluation rule *)
+| ppeval_lit (env : Environment) (l : Literal) (eff : SideEffectList) (id n : nat):
+  |env, id, ELit l, eff, S n| -pp> |id, inl (VLit l), eff|
+
+(* variable evaluation rule *)
+| ppeval_var (env:Environment) (s: Var) (eff : SideEffectList) (id : nat) (res : Value + Exception) n:
+  res = get_value env (inl s)
+->
+  |env, id, EVar s, eff, S n| -pp> |id, res, eff|
+
+(* Function Identifier evaluation rule *)
+| ppeval_funid (env:Environment) (fid : FunctionIdentifier) (eff : SideEffectList) 
+    (res : Value + Exception) (id n : nat):
+  res = get_value env (inr fid)
+->
+  |env, id, EFunId fid, eff, S n| -pp> |id, res, eff|
+
+(* Function evaluation *)
+| ppeval_fun (env : Environment) (vl : list Var) (e : Expression) (eff : SideEffectList) (id n : nat):
+  |env, id, EFun vl e, eff, S n| -pp> |S id, inl (VClos env [] id vl e), eff|
+
+| ppeval_let (env: Environment) (v : Var) (res : Value + Exception) (e1 e2 : Expression) (b : Value + Exception) (eff1 eff' eff'' : SideEffectList) (id id' id'' n : nat) :
+  |env, id, e1, eff1, n| -pp> |id', b, eff'| ->
+  |env, id', ALet v b e2 , eff', n| -aa> |id'', res, eff''|
+->
+  |env, id, ELet v e1 e2, eff1, S n| -pp> |id'', res, eff''|
+
+| ppeval_app env id id' id'' eff eff' eff'' exp params b res n:
+  |env, id, exp, eff, n| -pp> |id', b, eff'|
+  ->
+  |env, id', AApp1 b params, eff', n| -aa> |id'', res, eff''|
+->
+  | env, id, EApp exp params, eff, S n | -pp> |id'', res, eff''|
+
+(* call *)
+| ppeval_call env id id' id'' eff eff' eff'' res res' f params n:
+  | env, id, AList params (inl []), eff, n | -ll> | id', res, eff' | ->
+  | env, id', ACall f res, eff', n | -aa> | id'', res', eff'' |
+->
+  | env, id, ECall f params, eff,  S n | -pp> | id'', res', eff'' |
+
+(* try *)
+| ppeval_try env id id' id'' eff eff' eff'' e1 v1 e2 e3 vlist res res' n:
+  | env, id, e1, eff, n | -pp> |id', res, eff'| ->
+  | env, id', ATry res v1 e2 vlist e3, eff', n | -aa> |id'', res', eff''|
+->
+  | env, id, ETry e1 v1 e2 vlist e3, eff, S n | -pp> | id'', res' , eff'' |
+
+(* letrec *)
+| ppeval_letrec (env: Environment) (e b : Expression)  (l : list Var) (res : Value + Exception) (eff1 eff2 : SideEffectList) (f : FunctionIdentifier) (id id' n : nat) :
+  (
+     |append_funs_to_env [(f, (l, b))] env id, S id, e, eff1, n| -pp> | id', res, eff2|
+  )
+->
+  |env, id, ELetRec f l b e, eff1, S n| -pp> | id', res, eff2|
+
+where "| env , id , e , eff , counter | -pp> | id' , e' , eff' |" := (ppeval_expr env id e eff counter id' e' eff')
+with ppeval_list : Environment -> nat -> AuxList -> SideEffectList -> nat -> nat -> list Value + Exception -> SideEffectList -> Prop :=
+
+(* | peval_app2 env id id' id'' eff eff' eff'' v r rest vals res1 res2:
+  |env, id, r, eff| -p> |id', res1, eff'| ->
+  |env, id', AApp2 v rest (mk_result res1 vals), eff'| -a> |id'', res2, eff''|
+->
+  |env, id, AApp2 v (r::rest) (inl vals), eff| -a> |id'', res2, eff''| *)
+
+| ppeval_empty env id eff vals n:
+  | env, id, AList [] (inl vals), eff, S n | -ll> | id, inl vals, eff|
+
+| ppeval_list_cons env id id' id'' eff eff' eff'' r rest vals res res' n:
+  | env, id, r, eff , n| -pp> |id', res, eff'| ->
+  |env, id', AList rest (mk_result res vals), eff', n | -ll> | id'', res', eff''|
+->
+  | env, id, AList (r::rest) (inl vals), eff, S n | -ll> | id'', res', eff''|
+
+| ppeval_list_exc env id eff rest ex n:
+  | env, id, AList rest (inr ex), eff, S n | -ll> | id, inr ex, eff|
+
+where "| env , id , e , eff , counter | -ll> | id' , e' , eff' |" := (ppeval_list env id e eff counter id' e' eff')
+.
+
+Theorem ppeval_expr_increase :
+(forall n env id exp eff id' res eff' n1,
+  |env, id, exp, eff, n| -pp> |id', res, eff'| ->
+  n1 >= n ->
+  |env, id, exp, eff, n1| -pp> |id', res, eff'|
+)
+with ppeval_aux_increase :
+(forall n env id exp eff id' res eff' n1,
+  |env, id, exp, eff, n| -aa> |id', res, eff'| ->
+  n1 >= n ->
+  |env, id, exp, eff, n1| -aa> |id', res, eff'|
+)
+with ppeval_list_increase :
+(forall n env id exp eff id' res eff' n1,
+  |env, id, exp, eff, n| -ll> |id', res, eff'| ->
+  n1 >= n ->
+  |env, id, exp, eff, n1| -ll> |id', res, eff'|
+).
+Proof.
+{
+  induction n; intros.
+  * inversion H.
+  * destruct n1. inversion H0.
+    inversion H; subst.
+    - apply ppeval_lit.
+    - apply ppeval_var. auto.
+    - apply ppeval_funid. auto.
+    - apply ppeval_fun.
+    - eapply ppeval_let. apply IHn. exact H2. lia.
+      eapply ppeval_aux_increase. exact H7. lia.
+    - eapply ppeval_app. apply IHn. exact H2. lia.
+      eapply ppeval_aux_increase. exact H7. lia.
+    - eapply ppeval_call. eapply ppeval_list_increase. exact H2. 
+      lia. eapply ppeval_aux_increase. exact H7. lia.
+    - eapply ppeval_try. apply IHn. exact H2. lia.
+      eapply ppeval_aux_increase. exact H7. lia.
+    - eapply ppeval_letrec. apply IHn. exact H6. lia.
+}
+{
+  induction n; intros.
+  * inversion H.
+  * destruct n1. inversion H0.
+    inversion H; subst.
+    - eapply ppeval_app1_exc.
+    - eapply ppeval_app1_fin. eapply ppeval_list_increase. exact H2. lia.
+      eapply ppeval_aux_increase. exact H7. lia.
+    - eapply ppeval_app2_fin. auto.
+      eapply ppeval_expr_increase in H7. exact H7. lia.
+    - eapply ppeval_app2_exc1. auto.
+    - eapply ppeval_app2_exc2. auto.
+    - eapply ppeval_app2_exc.
+    - eapply ppeval_let_exc.
+    - eapply ppeval_let_fin. eapply ppeval_expr_increase in H6. exact H6. lia.
+    - eapply ppeval_call_fin. auto.
+    - eapply ppeval_call_exc.
+    - eapply ppeval_try1_fin. eapply ppeval_expr_increase in H6. exact H6. lia.
+    - eapply ppeval_try1_exc. eapply ppeval_expr_increase in H6. exact H6. lia.
+}
+{
+  induction n; intros.
+  * inversion H.
+  * destruct n1. inversion H0.
+    inversion H; subst.
+    - eapply ppeval_empty.
+    - eapply ppeval_list_cons. eapply ppeval_expr_increase. exact H2. lia.
+      eapply IHn. exact H7. lia.
+    - eapply ppeval_list_exc.
+}
+Qed.
+
+Theorem peval_ppeval :
+(forall env id exp eff id' res eff',
+  | env, id, exp, eff | -p> | id', res, eff' |
+->
+  exists n, |env, id, exp, eff, n| -pp> |id', res, eff'|)
+/\
+(forall env id exp eff id' res eff',
+  | env, id, exp, eff | -a> | id', res, eff' |
+->
+  exists n, |env, id, exp, eff, n| -aa> |id', res, eff'|)
+/\
+(forall env id exp eff id' res eff',
+  | env, id, exp, eff | -l> | id', res, eff' |
+->
+  exists n, |env, id, exp, eff, n| -ll> |id', res, eff'|)
+.
+Proof.
+  apply peval_ind; intros.
+  * exists 1. apply ppeval_lit.
+  * exists 1. apply ppeval_var. auto.
+  * exists 1. apply ppeval_funid. auto.
+  * exists 1. apply ppeval_fun.
+  * destruct H, H0. exists (S (x + x0)).
+    eapply ppeval_let.
+    - eapply ppeval_expr_increase. exact H. lia.
+    - eapply ppeval_aux_increase. exact H0. lia.
+  * destruct H, H0. exists (S (x + x0)).
+    eapply ppeval_app.
+    - eapply ppeval_expr_increase. exact H. lia.
+    - eapply ppeval_aux_increase. exact H0. lia.
+  * destruct H, H0. exists (S (x + x0)).
+    eapply ppeval_call.
+    - eapply ppeval_list_increase. exact H. lia.
+    - eapply ppeval_aux_increase. exact H0. lia.
+  * destruct H, H0. exists (S (x + x0)).
+    eapply ppeval_try.
+    - eapply ppeval_expr_increase. exact H. lia.
+    - eapply ppeval_aux_increase. exact H0. lia.
+  * destruct H. exists (S x).
+    eapply ppeval_letrec. auto.
+  * exists 1. apply ppeval_empty.
+  * destruct H, H0. exists (S (x + x0)).
+    eapply ppeval_list_cons.
+    - eapply ppeval_expr_increase. exact H. lia.
+    - eapply ppeval_list_increase. exact H0. lia.
+  * exists 1. eapply ppeval_list_exc.
+  * exists 1. eapply ppeval_app1_exc.
+  * destruct H, H0. exists (S (x + x0)).
+    eapply ppeval_app1_fin.
+    - eapply ppeval_list_increase. exact H. lia.
+    - eapply ppeval_aux_increase. exact H0. lia.
+  * destruct H. exists (S x).
+    eapply ppeval_app2_fin. auto. auto.
+  * exists 1. eapply ppeval_app2_exc1. auto.
+  * exists 1. eapply ppeval_app2_exc2. auto.
+  * exists 1. eapply ppeval_app2_exc.
+  * exists 1. eapply ppeval_let_exc.
+  * destruct H. exists (S x).
+    eapply ppeval_let_fin. auto.
+  * exists 1. eapply ppeval_call_fin. auto.
+  * exists 1. eapply ppeval_call_exc.
+  * destruct H. exists (S x). eapply ppeval_try1_fin.
+    auto.
+  * destruct H. exists (S x). eapply ppeval_try1_exc.
+    auto.
+Qed.
+
+
+
